src/functional_equations/example1.lean
@@ -64,7 +64,7 @@ begin
   exact bool.ff_ne_tt,
 end
 
-lemma single (x : nat) : hasElement [x] x := 
+lemma single {x : nat} : hasElement [x] x := 
   hasElement.step x []
 
 lemma two (x y : nat) : hasElement [x, y] y :=
@@ -80,7 +80,7 @@ begin
     change x ≠ y at h,
     -- rw hasElement.step_not_eq _ _ _ h, -- OK
     rw hasElement.step_not_eq,
-    { exact single y },
+    { exact @single y },
     { exact h },
   },
 end
@@ -97,20 +97,104 @@ end
 
 end hasElement
 
-
+variables {x : ℕ} {xs ys : list ℕ}
 
 constant union : list nat → list nat → list nat
 
-axiom union_base (xs : list nat) : union [] xs = xs
-axiom union_step₁ (x : nat) (xs ys : list nat) (h : hasElement ys x) :
+axiom union_base (xs : list nat) :
+  union [] xs = xs
+
+axiom union_step₁ (h : hasElement ys x) :
   union (x :: xs) ys = union xs ys
-axiom union_step₂ (x : nat) (xs ys : list nat) (h : hasElement ys x = ff) :
+
+axiom union_step₂ (h : hasElement ys x → false) :
   union (x :: xs) ys = union xs (x :: ys)
 
-lemma union_single (x : nat) : union [x] [x] = [x] :=
+
+lemma union_single : union [x] [x] = [x] :=
 begin
-  sorry,
+  have h₁ :                    union []  [x] = [x]          := union_base [x],
+  have h₂ : hasElement [x] x → union [x] [x] = union [] [x] := union_step₁,
+  have h₃ :                    union [x] [x] = union [] [x] := h₂ hasElement.single,
+  apply eq.trans h₃,
+  exact h₁,
 end
+
+lemma union_single' : union [x] [x] = [x] :=
+begin
+  rw union_step₁,
+  rw union_base,
+  apply hasElement.single,
+end
+
+#print notation >>=
+
+open tactic
+meta def trace_all : tactic unit :=
+   do n ← num_goals
+    , trace "num_goals ="
+    , trace n
+    , trace_state
+    , trace "---------------------------------------------"
+    , trace_result
+
+lemma union_single'' : union [x] [x] = [x] := by { 
+  apply eq.trans (union_step₁ hasElement.single),
+  trace_all,
+  sorry
+}
+
+meta def test_tactic : tactic unit :=
+do 
+  define `x (expr.const `nat [])
+, trace "-- after assert --"
+, trace_state
+, n ← get_local `n
+, trace (infer_type n)
+
+example (n : nat) : n = n := by { test_tactic, sorry }
+
+example : (1 = 2) → (2 = 3) → (3 = 1) := begin
+  assume h1 h2,
+  apply eq.symm,
+  apply eq.subst h2,
+  apply eq.subst h1,
+  apply eq.refl,
+  trace_result,
+  trace_call_stack,
+end
+
+example (a : nat) (b : bool) (c : int) : true := by {
+  do 
+    a ← get_local `a
+  , b ← get_local `b
+  , c ← get_local `c
+  , infer_type a >>= trace
+  , infer_type b >>= trace
+  , infer_type c >>= trace
+  , interactive.sorry
+}
+
+set_option trace.app_builder true
+-- set_option pp.all true
+
+example (a b c : ℕ) : true := by {
+  do
+    a ← get_local `a
+  , x ← mk_app `nat.succ [a] -- x : expr
+  , r ← to_expr ```(%%x + b * c + (λ n, n) 100) -- to_expr : pexpr → tactic expr
+  , trace r -- a.succ + b * c + (λ (n : ℕ), n) 100
+  , infer_type r >>= trace -- ℕ
+  , interactive.trivial -- or exact_dec_trivial
+}
+
+
+example (a b c : nat) (H1 : a = b) (H2 : b = c) : a = c :=
+by do
+  --  refine ```(eq.trans H1 _),
+   interactive.refine ```(eq.trans H1 _),
+   trace_state,
+   assumption
 
 end lemmas
 
@@ -129,7 +213,7 @@ end
 -- solve 3 = [[0], [1], [1]]
 -- solve 4 = [[0], [1], [1], [1, 2]]
 -- solve 5 = [[0], [1], [1], [1, 2], X], 
---    where X = (1 + [1, 2]) ∨ (1 + 1) = [2, 3] ∨ [2] = [2, 3]
+--    where X = (1 + [1, 2]) ∪ (1 + 1) = [2, 3] ∪ [2] = [2, 3]
 
 #print add_lt_add_of_le_of_lt -- a ≤ b → c < d → a + c < b + d
 
