src/palindromes.lean
@@ -1,4 +1,3 @@
-import data.list
 -- import .options
 
 set_option trace.simplify.rewrite true
@@ -10,21 +9,59 @@ inductive palindrome {α : Type} : list α → Prop
   palindrome ([x] ++ xs ++ [x])
 
 open list
+variable α : Type
 
-lemma reverse_palindrome {α : Type} (xs : list α)
+lemma rev_core_nil {ys : list α} : reverse_core ys nil = reverse ys := by rw reverse
+
+set_option pp.generalized_field_notation false
+
+namespace example_for_rev_append_cons
+def ys := [1,2,3,4]
+constant y : ℕ
+example : reverse (y :: ys) = reverse ys ++ [y] := rfl
+-- GOAL: ⊢ reverse (x :: xs ++ ys) = reverse ys ++ reverse (x :: xs)
+end example_for_rev_append_cons
+-- we have positive example means this lemma is potentially provable, and we can safely use sorry keyword
+
+lemma rev_append_cons (y : α) (ys : list α) : 
+  reverse (y :: ys) = reverse ys ++ [y] :=
+begin
+  induction ys,
+  case nil {
+    simp only [reverse, reverse_core, nil_append],
+    split; refl,
+  },
+  case cons : x ys ih {
+    sorry,
+  },
+end
+
+
+lemma reverse_append {xs ys : list α} :
+  reverse (xs ++ ys) = reverse ys ++ reverse xs :=
+begin
+  induction xs,
+  case nil {
+    rw [nil_append, reverse]; simp,
+    rw [reverse_core, append_nil],
+  },
+  case cons : x xs ih {
+    rw cons_append,
+    iterate 2 { rw rev_append_cons },
+    rw [←append_assoc, ih],
+  },
+end
+
+lemma reverse_palindrome (xs : list α)
     (hxs : palindrome xs) :
   palindrome (reverse xs) :=
 begin
   induction hxs,
-  case palindrome.nil {
-    exact palindrome.nil,
-  },
-  case palindrome.single {
-    exact palindrome.single hxs,
-  },
+  case palindrome.nil { exact palindrome.nil },
+  case palindrome.single { exact palindrome.single hxs },
   case palindrome.sandwich : x xs hxs ih {
     simp only [reverse, reverse_append],
-    apply palindrome.sandwich _ _ _,
-    exact ih,
+    -- type_check palindrome.sandwich _ (reverse xs) ih, -- palindrome ([?m_1] ++ reverse xs ++ [?m_1])
+    exact palindrome.sandwich x (reverse xs) ih,
   },
 end
