src/power_world.lean
@@ -1,3 +1,42 @@
+namespace hidden
+
+inductive mynat
+| zero : mynat
+| succ : mynat → mynat
+
+instance : has_zero mynat := ⟨mynat.zero⟩
+instance : has_one mynat := ⟨mynat.succ mynat.zero⟩
+
+def add : mynat → mynat → mynat
+| n 0 := n
+| n (mynat.succ m) := mynat.succ (add n m)
+
+instance : has_add mynat := ⟨add⟩
+
+@[pattern] def mul : mynat → mynat → mynat
+| n 0 := 0
+| n (mynat.succ m) := mul n m + n
+
+instance : has_mul mynat := ⟨mul⟩
+
+def pow : mynat → mynat → mynat
+| n 0 := 1
+| n (mynat.succ m) := pow n m * n
+
+instance : has_pow mynat mynat := ⟨pow⟩
+variables a b c : mynat
+
+lemma pow_zero : a ^ (0 : mynat) = 1 := by { dsimp [(^)], rw pow }
+lemma pow_succ : a ^ (mynat.succ b) = a ^ b * a := by { dsimp [(^)], rw pow }
+example : 5 * (1 : mynat)  = 5 := rfl
+lemma mul_one : a * (1 : mynat) = a := by {
+  -- dsimp [(*)],
+  -- unfold mul,
+  -- refl,
+  type_check mul,
+  sorry,
+}
+
 -- lemma zero_pow_succ (m : mynat) : (0 : mynat) ^ (succ m) = 0 :=
 -- begin
 --   let h := pow_succ 0 _,
@@ -16,14 +55,19 @@
 lemma one_pow (m : mynat) : (1 : mynat) ^ m = 1 :=
 begin
   have base := pow_zero 1,
-  have step := pow_succ 1 m,
-  rw mul_one at step,
+  have step := λ x, pow_succ 1 x,
+  apply mynat.rec_on m,
+  exact base,
+  intros a h₁,
+  rw (step a),
+  rw mul_one,
+  exact h₁,
 -- m : mynat,
 -- base : 1 ^ 0 = 1,
 -- step : 1 ^ succ m = 1 ^ m
 -- ⊢ 1 ^ m = 1
-  conv at step {
-    congr,
+  -- conv at step {
+    -- congr,
     -- 2 goals
     -- m : mynat,
     -- base : 1 ^ 0 = 1,
@@ -34,6 +78,7 @@ begin
     -- base : 1 ^ 0 = 1,
     -- step : 1 ^ succ m = 1 ^ m
     -- | 1 ^ m
-  }
-
+  -- },
 end
+
+end hidden
