src/tactics/my_method.lean
@@ -1,3 +1,7 @@
+import data.nat.modeq -- modular arithmetic
+import data.nat.prime -- prime number stuff
+import tactic.norm_num -- a tactic for fast computations
+import tactic.show_term
 
 namespace inequality_example
 -- http://wwwf.imperial.ac.uk/~buzzard/xena/natural_number_game/?world=9&level=1
@@ -27,3 +31,147 @@ begin
 end
 
 end inequality_example
+
+namespace hidden
+
+variables (x y z : bool)
+
+constant or : bool -> bool -> bool
+constant and : bool -> bool -> bool
+constant xor : bool -> bool -> bool
+constant imp : bool -> bool -> bool
+constant sheffer : bool -> bool -> bool
+constant not : bool -> bool
+
+axiom or_true : or tt x = tt
+axiom or_false : or ff x = x
+axiom and_true : and tt x = x
+axiom and_false : and ff x = ff
+axiom not_def : not x ≠ x
+
+lemma or_refl  : or  x x = x := by cases x; repeat {rw or_false  <|> rw or_true }
+lemma and_refl : and x x = x := by cases x; repeat {rw and_false <|> rw and_true}
+
+lemma or_comm : or x y = or y x :=
+begin
+  destruct x; intros h₁; rw h₁,
+  all_goals { 
+    try { rw or_false, },
+    try { rw or_true,  },
+    destruct y; intros h₂; rw h₂,
+  },
+  repeat { simp only [or_true, or_false] },
+end
+
+lemma and_comm : and x y = and y x := by cases x; cases y; repeat {rw and_false <|> rw and_true}
+
+#check nat.lt.base
+#check @nat.lt.step
+#check nat.le_succ
+#check @nat.less_than_or_equal.refl
+#check @nat.less_than_or_equal.step
+
+example : 1 + 1 > 1 := nat.lt.base 1
+lemma test : 20 > 10 := by repeat { apply nat.lt.base <|> apply nat.lt.step }
+#print test
+
+-- ∀ {p : ℕ → Prop} (a : ℕ), p 0 → (∀ (n : ℕ), (∀ (m : ℕ), m ≤ n → p m) → p n.succ) → p a
+
+
+lemma test_rewrite (A B : Prop) (h : A = B) : A -> B :=
+begin
+  have U : A → B, sorry,
+  rw h at U,
+  have do_nothing : (A → B) → A → B := id,
+  apply do_nothing,
+  -- apply eq.subst h, works
+  -- exact do_nothing, fail
+  exact h ▸ id,
+end
+
+example (n : nat) : n + 1 = 1 + n :=
+begin
+  type_check @nat.case_strong_induction_on,
+  apply @nat.case_strong_induction_on (λ n, n + 1 = 1 + n),
+  { refl },
+  intros n h,
+  change ∀ m, _ → _ = _ at h,
+  have h₂ := h n,
+  have h₃ : n ≤ n := @nat.less_than_or_equal.refl n,
+  have ih := h₂ h₃,
+  clear h₃ h₂ h,
+  change n.succ = 1 + n at ih,
+  rw ih,
+  change n + 1 = _ at ih,
+  rw add_assoc,
+  rw ih,
+end
+
+end hidden
+
+namespace example_logic_tactic
+
+
+-- split tactic
+
+open nat
+
+
+variables (a b : ℕ)
+example : (∀ k : ℕ, k > 1 → k ∣ a → ¬ (k ∣ b) ) → coprime a b := coprime_of_dvd
+example : coprime a b → gcd a b = 1 := coprime.gcd_eq_one
+example : (∀ k : ℕ, k > 1 → k ∣ a → ¬ (k ∣ b) ) → gcd a b = 1 := λ h, coprime.gcd_eq_one $ coprime_of_dvd h
+
+example : 5 ≡ 1 [MOD 4] := rfl
+example (a b c d m : nat):
+  a ≡ b [MOD m] → c ≡ d [MOD m] → a * c ≡ b * d [MOD m] :=
+  @modeq.modeq_mul m a b c d
+
+
+lemma prime_2 : prime 2 := dec_trivial
+
+lemma prime_5 : prime 5 := by norm_num
+
+#print prime_5
+-- (id
+--    (eq_true_intro
+--       (norm_num.is_prime_helper 5 (norm_num.lt_one_bit1 2 (bit0_pos zero_lt_one))
+--          (norm_num.min_fac_helper_5 2 1 9
+--             (norm_num.mul_bit1_bit1 1 1 1 2 4 (one_mul 1) norm_num.one_succ
+--                (norm_num.add_bit0_bit0 1 1 2 norm_num.one_succ))
+--             (norm_num.lt_bit1_bit1 2 4 (norm_num.lt_bit0_bit0 1 2 (norm_num.lt_one_bit0 1 (le_refl 1))))
+--             (norm_num.min_fac_helper_0 2 (bit0_pos zero_lt_one)))))).mpr
+--   trivial
+
+#eval factors 1023 -- [3, 11, 31]
+#eval (factors 1024).length -- 10
+
+open tactic 
+meta def show_term' :=
+  do
+    g :: rest ← get_goals,
+    trace get_goals
+
+
+example {P Q R : Prop} (h₁ : Q → P) (h₂ : R) (h₃ : R → Q) : P ∧ R :=
+by show_term { tactic.tauto }
+
+lemma test_split (A B : Prop) : A ∧ B → B ∧ A := by {
+  intros h,
+  split,
+  show_term',
+  all_goals { sorry },
+}
+
+meta def split' : tactic 
+
+meta def split_unit : tactic unit := 
+  concat_tags split'
+
+
+
+
+
+
+end example_logic_tactic
+
