src/tactics/back_chaining1.lean
@@ -6,7 +6,15 @@ attribute [intro] Huq Hur Hus Hut
 
 open tactic
 
+set_option back_chaining.max_depth 1
+set_option trace.tactic.back_chaining true
+
 definition lemma1 (p : P) : Q := by back_chaining
 definition lemma2 (p : P) : R := by back_chaining
 definition lemma3 (p : P) : S := by back_chaining
 definition lemma4 (p : P) : T := by back_chaining
+
+#print lemma1 -- λ (p : P), Hpq p
+#print lemma2 -- λ (p : P), Hqr (Hpq p)
+#print lemma3 -- λ (p : P), Hrs (Hqr (Hpq p))
+#print lemma4 -- λ (p : P), Hst (Hrs (Hqr (Hpq p)))
